\newcommand{\maxwell}
{
\begin{align}
\nabla\times {\mathbf{E}}&=-\frac{\partial {\mathbf{B}}}{\partial t}  \\
\nabla\times {\mathbf{H}}&={\mathbf{J}}+\frac{\partial {\mathbf{D}}}{\partial t}  \\
\nabla\cdot {\mathbf{B}}&=0  \\
\nabla\cdot {\mathbf{D}}&=\rho 
\label{eq:maxwell}
\end{align}
}


\newcommand{\maxwella}
{\begin{align}
{\mathbf{B}}&=\mu {\mathbf{H}}  \\
{\mathbf{D}}&=\varepsilon {\mathbf{E}}  \\
{\mathbf{J}}&=\sigma {\mathbf{E}} 
\label{eq:maxwella}
\end{align}
}


\newcommand{\ect}
{
\begin{equation}
   \nabla \cdot\left(\varepsilon \nabla \varphi \right)=0
\label{eq:ect}
\end{equation}
}

\newcommand{\ecrt}
{
\begin{equation}
  \nabla \cdot\left[(\sigma +j\omega \varepsilon )\nabla \varphi \right]=0
\label{eq:ecrt}
\end{equation}}

\newcommand{\ectb}
{
\begin{equation}
\left\{
\begin{array}{rl}
    \varphi_{\Gamma_e}=&V_e\\
    \varphi_{\Gamma_m}=&0\\
    \varphi_{\Gamma_{s}}=&0\\
\end{array}
\right.  
\label{eq:ectb}
\end{equation}
}


\newcommand{\capacitance}
{
\begin{equation}
  C=\frac{Q}{V_e}=-\frac{1}{V_e}\int_{\Omega_m}\varepsilon(x,y,z)\nabla\varphi(x,y,z) d\Omega
\label{eq:capacitance}  
\end{equation}
}

\newcommand{\emt}
{
\begin{equation}
  \nabla\times \left[\left(\nabla \times \frac{\mathbf{B}}{\mu}\right)/\sigma\right]=-j\omega \mathbf{B}  
  \label{eq:emt}
\end{equation}
}

\newcommand{\emta}
{
  \begin{equation}
  \nabla^2\mathbf{A}+j\omega\mu\sigma \mathbf{A}=\mu \mathbf{J}
  \label{eq:emta}
\end{equation}
}


\newcommand{\deltaz}
{
  \begin{align}
    \Delta Z &= \frac{1}{I^2}\int_{\Omega}j\omega(\mu_x-\mu_0)\mathbf{H}_x\cdot\mathbf{H}_0 \nonumber\\
    &-(\sigma_x-\sigma_0+j\omega\varepsilon_x-j\omega\varepsilon_0)\mathbf{E}_x\cdot\mathbf{E}_0 d\Omega
    \label{eq:deltaz}
  \end{align}
}


\newcommand{\snr}
{
  \begin{equation}
    \mathbf{SNR} = -20\lg\left[\frac{1}{\mu}\sqrt{\frac{1}{n}\sum\limits_{i=1}^{n}(x_i-\mu)^{2}}\right]
    \label{eq:snr}
  \end{equation}
}


\newcommand{\snrd}
{
  \begin{equation}
    \mathbf{SNR_\Delta} = -20\lg\left[\frac{1}{|\mu_h-\mu_l|}\sqrt{\frac{1}{n}\sum\limits_{i=1}^{n}(x_i-\mu_h)^{2}}\right]    \label{eq:snrd}
  \end{equation}
}

\newcommand{\corrcoe}
{
  \begin{equation}
    r=\frac{\sum_{i=1}^{N}\left(\hat{\mathbf{g}}_{i}-\overline{\hat{\mathbf{g}}}\right)\left(\mathbf{g}_{i}-\overline{\mathbf{g}}\right)}{\sqrt{\sum_{i=1}^{N}\left(\hat{\mathbf{g}}_{i}-\overline{\hat{\mathbf{g}}}\right)^{2} \sum_{i=1}^{N}\left(\mathbf{g}_{i}-\overline{\mathbf{g}}\right)^{2}}}
    \label{eq:corrcoe}
  \end{equation}
}

\newcommand{\rmse}{
  \begin{equation}
    \mathbf{RMSE} = \sqrt{\frac{1}{N}\sum_{i=1}^{N}(\hat{\delta}_{i} - \delta_{i})^2}
    \label{eq:rmse}
  \end{equation}
}

\newcommand{\emap}
{
  \begin{equation}\label{eq:normc}
    \delta_h^p = \frac{C_{e}-C_{l}}{C_{h}-C_{l}}
    \end{equation}
}

\newcommand{\emas}
{
  \begin{equation}\label{eq:emas}
    \delta_h^s = \frac{C_{h}}{C_{e}}\frac{(C_{e}-C_{l})}{(C_{h}-C_{l})}=\left(\frac{C_h}{C_e}\right)\delta_h^p
  \end{equation}
}

\newcommand{\emamg}
{
  \begin{equation}\label{eq:emamg}
    \delta_{h}^{MG}
    =\frac{(C_{h}+2C_{l})}{(C_{e}+2C_{l})}\frac{(C_{e}-C_{l})}{(C_{h}-C_{l})}
    =\left(\frac{C_{h}+2C_{l}}{C_{e}+2C_{l}}\right) \delta_h^p
    \end{equation}
}

\newcommand{\emabo}{
  \begin{equation}\label{eq:emabo}
  \delta_h^{Bo}=
  \frac{(C_h+2C_e)}{3C_e}\frac{(C_{e}-C_{l})}{(C_{h}-C_{l})}
  =\left(\frac{2C_{e}+C_{h}}{3C_{e}}\right)\delta_h^p
\end{equation}
}

\newcommand{\emabr}{
  \begin{equation}\label{eq:emabr}
  \delta_h^{Br}= \frac{C_{e}+C_{h}}{2C_{e}}\frac{(C_{e}-C_{l})}{(C_{h}-C_{l})}
  =\left(\frac{C_{e}+C_{h}}{2C_{e}}\right)\delta_h^p
\end{equation}
}

\newcommand{\emft}{
  \begin{equation} \label{eq:emft}
    \nabla \cdot \sigma \nabla \varphi = \nabla \cdot \sigma (\vec {v} \times \vec {B}), 
\end{equation}
}


\newcommand{\emftb}{
  \begin{align*} 
    \frac {\partial \varphi}{\partial \hat {n}}=&0, \quad \vec {r} \in \partial \Omega, 
    \\ 
    \vec {v}=&0, \quad \vec {r} \in \partial \Omega _{\mathrm{wall}}, 
    \\ 
    \vec {B}=&0, \quad \vec {r} \in \partial \Omega _{\mathrm{ends}}, 
  \end{align*}  
}


